{
 "cells": [
  {
   "cell_type": "markdown",
   "id": "ac6ab498",
   "metadata": {},
   "source": [
    "# Cramer's rule\n",
    "\n",
    "**Cramer's rule** is an explicit rule for calculating the solution to a system of linear equations using determinants.\n",
    "\n",
    "::::{admonition} Theorem: Cramer's rule\n",
    ":class: important\n",
    ":name: cramers-rule-theorem\n",
    "\n",
    "The solution to a non-singular linear system of equations of the form $A\\mathbf{x}=\\mathbf{b}$ can be calculated using Cramer's rule which is\n",
    "\n",
    ":::{math}\n",
    ":label: cramers-rule-equation\n",
    "\n",
    "x_i = \\frac{\\det(A_i)}{\\det(A)},\n",
    ":::\n",
    "\n",
    "where $A_i$ is a matrix obtained by replacing column $i$ of $A$ with $\\mathbf{b}$.\n",
    "\n",
    "::::\n",
    "\n",
    "**Proof**\n",
    "\n",
    "*Consider the solution to the linear system $A\\mathbf{x} = \\mathbf{b}$ where $A$ is non-singular then the solution for the first variable $x_1$ is*\n",
    "\n",
    "\\begin{align*}\n",
    "    x_1 = \\det \n",
    "    \\begin{pmatrix} \n",
    "        x_1 & 0 & \\cdots & 0 \\\\\n",
    "        x_2 & 1 & \\cdots & 0 \\\\\n",
    "        \\vdots & \\vdots & \\ddots & \\vdots \\\\\n",
    "        x_n & 0 & \\cdots & 1\n",
    "    \\end{pmatrix} = \\det(X_1).\n",
    "\\end{align*}\n",
    "\n",
    "*Since $\\mathbf{x} = A^{-1}\\mathbf{b}$ and $I = A^{-1}A$ then the matrix $X_1$ can be written as*\n",
    "\n",
    "\\begin{align*}\n",
    "    X_1 = \\begin{pmatrix} A^{-1}\\mathbf{b} & A^{-1} \\mathbf{a}_2 & \\cdots & A^{-1} \\mathbf{a}_n \\end{pmatrix},\n",
    "\\end{align*}\n",
    "\n",
    "*where $\\mathbf{a}_i$ is the $i$th column of $A$. Since $A_1$ in equation {eq}`cramers-rule-equation` is $A_1 = \\begin{pmatrix} \\mathbf{b} & \\mathbf{a}_2 & \\cdots & \\mathbf{a}_n \\end{pmatrix}$ then $X_1 = A^{-1}A_1$. Using the property of determinant where the determinant of a product of two matrices is equal to the product of the determinants  then*\n",
    "\n",
    "\\begin{align*}\n",
    "    x_1 = \\det(X_1) = \\det(A^{-1}A_1) = \\det(A^{-1})\\det(A_1) = \\frac{\\det(A_1)}{\\det(A)}.\n",
    "\\end{align*}\n",
    "\n",
    "*Doing similar for the other variables completes the proof.* <div style=\"text-align: right\"> &#9633; </div>\n",
    "\n",
    "\n",
    ":::::{admonition} Example 2.3\n",
    ":class: seealso\n",
    ":name: cramers-rule-example\n",
    "\n",
    "Solve the following systems of linear equations using Cramer's rule\n",
    "\n",
    "::::{grid}\n",
    "\n",
    ":::{grid-item}\n",
    "(i) &emsp; $\\begin{array}{rl}\n",
    "    3x_1 - 2x_2 &= -4, \\\\\n",
    "    x_1 - 3x_2 &= 1.\n",
    "\\end{array}$\n",
    ":::\n",
    "\n",
    ":::{grid-item}\n",
    "(ii) &emsp; $\\begin{array}{rl}\n",
    "    -2x_1 - 3x_2 - x_3 &= -5, \\\\\n",
    "    -4x_1 + 4x_2 + 3x_3 &= -20, \\\\\n",
    "    -3x_1 &= -12.\n",
    "\\end{array}$\n",
    ":::\n",
    "\n",
    "::::\n",
    "\n",
    "::::{dropdown} Solution\n",
    "\n",
    "(i) $A = \\begin{pmatrix} 3 & -2 \\\\ 1 & -3 \\end{pmatrix}$ and $\\mathbf{b} = \\begin{pmatrix} -4 \\\\ 1 \\end{pmatrix}$\n",
    "\n",
    "\\begin{align*}\n",
    "    x_1 &= \\frac{\n",
    "    \\begin{vmatrix} -4 & -2 \\\\ 1 & -3 \\end{vmatrix}}\n",
    "    {\\begin{vmatrix} 3 & -2 \\\\ 1 & -3 \\end{vmatrix}} = \\frac{14}{-7} = -2,  \\\\\n",
    "    \\\\\n",
    "    x_2 &= \\frac{\\begin{vmatrix} 3 & -4 \\\\ 1 & 1 \\end{vmatrix}}{-7} = \n",
    "    \\frac{7}{-7} = -1.\n",
    "\\end{align*}\n",
    "\n",
    "Check solution:\n",
    "\n",
    "\\begin{align*}\n",
    "    A\\mathbf{x} = \\begin{pmatrix} 3 & -2 \\\\ 1 & -3 \\end{pmatrix}\n",
    "    \\begin{pmatrix} -2 \\\\ -1 \\end{pmatrix} =\n",
    "    \\begin{pmatrix} -4 \\\\ 1 \\end{pmatrix} = \\mathbf{b}.\n",
    "\\end{align*}\n",
    "\n",
    "(ii) $A = \\begin{pmatrix} -2 & -3 & -1 \\\\ -4 & 4 & 3 \\\\ -3 & 0 & 0 \\end{pmatrix}$ and $\\mathbf{b} = \\begin{pmatrix} -5 \\\\ -20 \\\\ -12 \\end{pmatrix}$\n",
    "\n",
    "\\begin{align*}\n",
    "    x_1 &= \\frac{\n",
    "    \\begin{vmatrix}-5 & -3 & -1 \\\\ -20 & 4 & 3 \\\\ -12 & 0 & 0 \\end{vmatrix}}\n",
    "    {\\begin{vmatrix} -2 & -3 & -1 \\\\ -4 & 4 & 3 \\\\ -3 & 0 & 0 \\end{vmatrix}}\n",
    "    = \\frac{-12\n",
    "    \\begin{vmatrix} -3 & -1 \\\\ 4 & 3 \\end{vmatrix}}\n",
    "    {-3\\begin{vmatrix} -3 & -1 \\\\ 4 & 3 \\end{vmatrix}} \\\\\n",
    "    &= \\frac{-12(-5)}{-3(-5)} = \\frac{60}{15} = 4,\\\\ \\\\\n",
    "    x_2 &= \\frac{\n",
    "    \\begin{vmatrix} -2 & -5 & -1 \\\\ -4 & -20 & 3 \\\\ -3 & -12 & 0 \\end{vmatrix}}{15} \n",
    "    = \\frac{-\\begin{vmatrix} -4 & -20 \\\\ -3 & -12 \\end{vmatrix} \n",
    "    - 3\\begin{vmatrix}-2 & -5 \\\\ -3 & -12 \\end{vmatrix}}{15}  \\\\\n",
    "    &= \\frac{12 - 3(9)}{15} = \\frac{-15}{15} = -1, \\\\ \\\\\n",
    "    x_3 &= \\frac{\n",
    "    \\begin{vmatrix} -2 & -3 & - 5 \\\\ -4 & 4 & -20 \\\\ -3 & 0 & -12 \\end{vmatrix}}{15}\n",
    "    =\\frac{-3\\begin{vmatrix} -3 & -5 \\\\ 4 & -20 \\end{vmatrix} - \n",
    "    12\\begin{vmatrix} -2 & -3 \\\\ -4 & 4 \\end{vmatrix}}{15} \\\\\n",
    "    & = \\frac{-3(80) - 12(-20)}{15} = \\frac{0}{15} = 0.\n",
    "\\end{align*}\n",
    "\n",
    "Check solution:\n",
    "\n",
    "\\begin{align*}\n",
    "    A\\mathbf{x} = \n",
    "    \\begin{pmatrix} -2 & -3 & -1 \\\\ -4 & 4 & 3 \\\\ -3 & 0 & 0 \\end{pmatrix}\n",
    "    \\begin{pmatrix} 4 \\\\ -1 \\\\ 0 \\end{pmatrix} =\n",
    "    \\begin{pmatrix} -5 \\\\ -20 \\\\ -12 \\end{pmatrix} = \\mathbf{b}.\n",
    "\\end{align*}\n",
    "\n",
    "::::\n",
    "\n",
    ":::::"
   ]
  }
 ],
 "metadata": {
  "kernelspec": {
   "display_name": "Python 3",
   "language": "python",
   "name": "python3"
  },
  "language_info": {
   "codemirror_mode": {
    "name": "ipython",
    "version": 3
   },
   "file_extension": ".py",
   "mimetype": "text/x-python",
   "name": "python",
   "nbconvert_exporter": "python",
   "pygments_lexer": "ipython3",
   "version": "3.8.3"
  }
 },
 "nbformat": 4,
 "nbformat_minor": 5
}